Rename: lift -> flipBind

Dpda/Basic.lean
@@ -4,13 +4,16 @@ import Mathlib.Data.Fintype.Basic
 import Mathlib.Data.Fintype.Prod
 import Mathlib.Data.Fintype.Option
 
-def lift {α} (f : α → Option α) : Option α → Option α :=
+
+-- Basically (fun u => u >>= f) but avoid using `>>=` directly
+-- def flipBind {α} : (α → Option α) →  Option α → Option α := flip bind
+def flipBind {α} (f : α → Option α) : Option α → Option α :=
   fun u =>
     match u with
     | none => none
     | some (a: α) => f a
 
-lemma repeat_lift_map α β γ
+lemma repeat_flipBind_map α β γ
   (η_o : α → β)
   (pick: γ → (α → Option α))
   (η_f : γ → (β → Option β))
@@ -18,12 +21,12 @@ lemma repeat_lift_map α β γ
   (th : ∀ a, ((pick g) a).map η_o = (η_f g) (η_o a))
   (n : Nat)
   (a : α) :
-  Nat.repeat (lift (η_f g)) n (some (η_o a)) = (Nat.repeat (lift (pick g)) n (some a)).map η_o := by
+  Nat.repeat (flipBind (η_f g)) n (some (η_o a)) = (Nat.repeat (flipBind (pick g)) n (some a)).map η_o := by
   induction n with
   | zero => rfl
   | succ n ih =>
-    simp only [Nat.repeat, lift, ih]
-    cases h : Nat.repeat (lift (pick g)) n (some a) with
+    simp only [Nat.repeat, flipBind, ih]
+    cases h : Nat.repeat (flipBind (pick g)) n (some a) with
     | none => rfl
     | some a' =>
       simp only [Option.map_some]
